Projects/Esolangs/Cornucopia/Programs/Prog1.lean
@@ -1,217 +1,610 @@
-import Projects.Esolangs.Cornucopia.Basic
+import Projects.Esolangs.Cornucopia.Programs.Common
 
 attribute [-simp] List.getElem!_eq_getElem?_getD
 
-namespace Esolangs.Cornucopia
+namespace Esolangs.Cornucopia.Prog₁
 
--- def refZero : Expr :=
---   .call (.custom 1) []
--- 
--- def refOne : Expr :=
---   .call (.custom 2) []
--- 
--- def exprZero : Expr :=
---   .call (.builtin .sub) [refZero, refZero]
--- 
--- def exprOne : Expr :=
---   .call (.builtin .succ) [refZero]
--- 
--- def exprNot : Expr :=
---   .call (.builtin .sub) [refOne, .arg 0]
--- 
--- def exprBool : Expr :=
---   .call (.custom 3) [.call (.custom 3) [.arg 0]]
--- 
--- def exprAdd : Expr :=
---   .call (.builtin .sub)
---   [ .call (.builtin .sub)
---     [ .call (.builtin .sub)
---       [ .call (.builtin .succ) [.call (.builtin .succ) [
---           .call (.custom 5)
---             [ .call (.builtin .sub) [.arg 0, refOne]
---             , .call (.builtin .sub) [.arg 1, refOne]
---             ]
---         ]]
---       , .call (.custom 3) [.arg 0]
---       ]
---     , .call (.custom 3) [.arg 1]
---     ]
---   , .call (.custom 5) [refZero, refZero]
---   ]
--- 
--- -- def refOneAlt : Expr :=
--- --   .call (.custom 6) []
--- -- 
--- -- def exprOneAlt : Expr :=
--- --   .call (.builtin .sub)
--- --   [ .call (.builtin .succ) [.custom 6]
--- --   ]
--- 
--- def exprMain₁ : Expr :=
---   exprId
--- 
--- def prog₁ : Prog where
---   defs := [
---     ⟨1, exprMain₁⟩,
---     ⟨0, exprZero⟩,
---     ⟨0, exprOne⟩,
---     ⟨1, exprNot⟩,
---     ⟨1, exprBool⟩,
---     ⟨2, exprAdd⟩,
---   ]
--- 
--- def prog₁FS : List (List ℕ → ℕ) :=
---   [ fn 1 λ xs => xs[0]!
---   , fn 0 λ _ => 0
---   , fn 0 λ _ => 1
---   , fn 1 λ xs => if xs[0]! = 0 then 1 else 0
---   , fn 1 λ xs => if xs[0]! = 0 then 0 else 1
---   , fn 2 λ xs => xs[0]! + xs[1]!
---   ]
--- 
--- -- #check 0 #exit
--- 
--- -----
--- 
--- @[simp]
--- theorem wf_expr_prog₁_main₁ : exprMain₁.WF prog₁ 1 := by
---   simp [exprMain₁]
--- 
--- @[simp]
--- theorem wf_def_prog₁_main₁ : Def.WF prog₁ ⟨1, exprMain₁⟩ := by
---   simp [Def.WF]
--- 
--- -- #check 0 #exit
--- 
--- theorem exprAdd_aux {f : ℕ → ℕ → ℕ} (h : ∀ x y, f x y = f (x - 1) (y - 1) + 2 -
--- (if x = 0 then 1 else 0) - (if y = 0 then 1 else 0) - f 0 0) : f = (· + ·) := by
---   ext x y
---   have h₁ : f 0 0 = 0
---   · specialize h 0 0
---     simpa using h
---   induction x generalizing y
---   · specialize h 0
---     simp at h
---     induction y
---     · specialize h 0
---       simpa using h
---     nm y ih
---     specialize h (y + 1)
---     simp_all
---   nm x ih
---   specialize h (x + 1) y
---   simp_all
---   specialize ih (y + 1)
---   grind
--- 
--- -- #check 0 #exit
--- 
--- @[simp] theorem length_defs_prog₁ : prog₁.defs.length = 6 := rfl
--- 
--- @[simp] theorem prog₁_arity_0 : prog₁.arity 0 = 1 := rfl
--- @[simp] theorem prog₁_arity_1 : prog₁.arity 1 = 0 := rfl
--- @[simp] theorem prog₁_arity_2 : prog₁.arity 2 = 0 := rfl
--- @[simp] theorem prog₁_arity_3 : prog₁.arity 3 = 1 := rfl
--- @[simp] theorem prog₁_arity_4 : prog₁.arity 4 = 1 := rfl
--- @[simp] theorem prog₁_arity_5 : prog₁.arity 5 = 2 := rfl
--- 
--- @[simp]
--- theorem wf_prog₁_refZero {n} : refZero.WF prog₁ n := by
---   simp [refZero]
--- 
--- @[simp]
--- theorem wf_expr_prog₁_exprZero {n} : exprZero.WF prog₁ n := by
---   simp [exprZero]
--- 
--- @[simp]
--- theorem wf_prog₁_refOne {n} : refOne.WF prog₁ n := by
---   simp [refOne]
--- 
--- @[simp]
--- theorem wf_expr_prog₁_exprOne {n} : exprOne.WF prog₁ n := by
---   simp [exprOne]
--- 
--- @[simp]
--- theorem wf_expr_prog₁_exprNot {n} : exprNot.WF prog₁ n ↔ 1 ≤ n := by
---   simp [exprNot]; omega
--- 
--- @[simp]
--- theorem wf_expr_prog₁_exprBool {n} : exprBool.WF prog₁ n ↔ 1 ≤ n := by
---   simp [exprBool]; omega
--- 
--- @[simp]
--- theorem wf_expr_prog₁_exprAdd {n} : exprAdd.WF prog₁ n ↔ 2 ≤ n := by
---   simp [exprAdd]; omega
--- 
--- -- #check 0 #exit
--- 
--- @[simp]
--- theorem compatible_prog₁_prog₁FS : prog₁.Compatible prog₁FS := by
---   unfold prog₁FS; constructor <;> simp
---   all_goals
---     intro i h xs h₁
---     obtain rfl | rfl | rfl | rfl | rfl | rfl :
---       i = 0 ∨ i = 1 ∨ i = 2 ∨ i = 3 ∨ i = 4 ∨ i = 5 := by omega
---   iterate 6 simp at h₁; simp [fn] <;> try grind
---   all_goals nth_rw 1 [prog₁]; (try simp at h₁); simp [fn, h₁]
---   · simp [exprMain₁, exprId]
---   · simp [exprZero]
---   · simp [exprOne, refZero, fn]
---   · simp [exprNot, refOne, fn]; grind
---   · simp [exprBool, fn]; grind
---   · simp [exprAdd, fn]; rw! [xs.eq_getElem_of_length_eq_two h₁]
---     simp; generalize xs[0] = x; generalize xs[1] = y; clear h₁ xs
---     simp [refOne, refZero, fn]; cases x; cases y <;> rfl; nm x
---     simp; cases y; rfl; nm y; simp; omega
--- 
--- @[simp, instance]
--- theorem wf_prog₁ : prog₁.WF := by
---   constructor; rintro ⟨⟩; rfl; nth_rw 1 [prog₁]; simp
---   use prog₁FS, (by simp); unfold prog₁FS
---   rintro fs ⟨h₁, h₂, h₃⟩; simp at h₁ h₂ h₃
---   have h_zero : fs[1]! [] = 0
---   · specialize @h₃ 1 (by omega) [] (by simp)
---     simp [prog₁, exprZero] at h₃; exact h₃
---   have h_one : fs[2]! [] = 1
---   · specialize @h₃ 2 (by omega) [] (by simp)
---     simp [prog₁, exprOne, refZero] at h₃; grind
---   have h_not : ∀ ⦃x⦄, fs[3]! [x] = if x = 0 then 1 else 0
---   · intro x; specialize @h₃ 3 (by omega) [x] (by simp)
---     simp [prog₁, exprNot, refOne] at h₃; grind
---   have h_bool : ∀ ⦃x⦄, fs[4]! [x] = if x = 0 then 0 else 1
---   · intro x; specialize @h₃ 4 (by omega) [x] (by simp)
---     simp [prog₁, exprBool] at h₃; grind
---   have h_add : ∀ ⦃x y⦄, fs[5]! [x, y] = x + y
---   · intro x y; specialize @h₃ 5 (by omega)
---     simp [prog₁, exprAdd, refOne, refZero] at h₃
---     simp [h_zero, h_one, h_not] at h₃
---     replace h₃ : ∀ x y, fs[5]! [x, y] = fs[5]! [x - 1, y - 1] + 2 -
---       (if x = 0 then 1 else 0) - (if y = 0 then 1 else 0) - fs[5]! [0, 0]
---     · intro x y; specialize @h₃ [x, y]; simp at h₃; omega
---     have h₄ := exprAdd_aux (f := λ x y => fs[5]! [x, y]) (by grind); grind
---   rw [List.ext_getElem!_iff]; simp [h₁]; intro i h₄; ext xs
---   specialize @h₂ i (by omega); specialize @h₃ i (by omega)
---   specialize @h₂ xs; specialize @h₃ xs
---   obtain rfl | rfl | rfl | rfl | rfl | rfl :
---     i = 0 ∨ i = 1 ∨ i = 2 ∨ i = 3 ∨ i = 4 ∨ i = 5 := by omega
---   all_goals simp [prog₁, fn] at h₂ h₃ ⊢
---   · split_ifs with H
---     · specialize h₃ H; simp [exprMain₁, exprId] at h₃; grind
---     · specialize h₂ H; grind
---   · simp [exprZero] at h₃; grind
---   · simp [exprOne] at h₂ h₃; grind
---   · simp [exprNot, refOne] at h₂ h₃; grind
---   · simp [exprBool] at h₂ h₃; grind
---   · simp [exprAdd, refOne, refZero] at h₂ h₃; grind
--- 
--- @[simp]
--- theorem fs_prog₁ : prog₁.fs = prog₁FS :=
---   Prog.fs_eq_of_compatible compatible_prog₁_prog₁FS
--- 
--- @[simp]
--- theorem eval_prog₁ {i xs} : prog₁.eval i xs = prog₁FS[i]! xs := by
---   simp [Prog.eval]
--- 
--- @[simp]
--- theorem run_prog₁ {x} : prog₁.run x = x := by
---   simp [Prog.run, Prog.eval, prog₁FS, fn]
+def defNot : Def :=
+  ⟨1, .call subName [one, .arg 0]⟩
+
+def defBool : Def :=
+  ⟨1, .call "not" [.call "not" [.arg 0]]⟩
+
+def exprAdd : Expr :=
+  .call subName
+  [ .call subName
+    [ .call subName
+      [ .call succName [.call succName [
+          .call "add"
+            [ .call subName [.arg 0, one]
+            , .call subName [.arg 1, one]
+            ]
+        ]]
+      , .call "not" [.arg 0]
+      ]
+    , .call "not" [.arg 1]
+    ]
+  , .call "add" [zero, zero]
+  ]
+
+def defAdd : Def :=
+  ⟨2, exprAdd⟩
+
+def exprIte : Expr :=
+  .call subName
+  [ .call subName
+    [ .call subName
+      [ .call succName
+        [ .call "ite"
+          [ .arg 0
+          , .call subName [.arg 1, one]
+          , .call subName [.arg 2, one]
+          ]
+        ]
+      , .call subName
+        [ .call "bool" [.arg 0]
+        , .arg 1
+        ]
+      ]
+    , .call subName
+      [ .call "not" [.arg 0]
+      , .arg 2
+      ]
+    ]
+  , .call "ite" [.arg 0, zero, zero]
+  ]
+
+def defIte : Def :=
+  ⟨3, exprIte⟩
+
+def defs : List (String × Def) :=
+  [ (mainName, defId)
+  , ("0", defZero)
+  , ("1", defOne)
+  , ("not", defNot)
+  , ("bool", defBool)
+  , ("add", defAdd)
+  , ("ite", defIte)
+  ]
+
+def fs : List (String × (List ℕ → ℕ)) :=
+  [ (mainName, fn 1 (·[0]!))
+  , ("0", fn 0 λ _ => 0)
+  , ("1", fn 0 λ _ => 1)
+  , ("not", fn 1 λ xs => if xs[0]! = 0 then 1 else 0)
+  , ("bool", fn 1 λ xs => if xs[0]! = 0 then 0 else 1)
+  , ("add", fn 2 λ xs => xs[0]! + xs[1]!)
+  , ("ite", fn 3 λ xs => if xs[0]! = 0 then xs[2]! else xs[1]!)
+  ]
+
+def fsMap : Map String (List ℕ → ℕ) :=
+  builtinFs ∪ .ofList fs
+
+def prog : Prog :=
+  .ofDefs defs
+
+-- #check 0 #exit
+
+-----
+
+@[simp]
+theorem nodup_defs : defs.map (·.1) |>.Nodup := by
+  decide
+
+@[simp]
+theorem nodup_fs : fs.map (·.1) |>.Nodup := by
+  decide
+
+@[instance, simp]
+theorem wfBuiltins_prog : prog.WFBuiltins := by
+  apply Prog.wfBuiltins_ofDefs; decide
+
+@[simp] theorem arity_defNot : defNot.arity = 1 := rfl
+@[simp] theorem arity_defBool : defBool.arity = 1 := rfl
+@[simp] theorem arity_defAdd : defAdd.arity = 2 := rfl
+@[simp] theorem arity_defIte : defIte.arity = 3 := rfl
+
+-- #check 0 #exit
+
+@[simp]
+theorem hasDef_prog_iff {name} : prog.HasDef name ↔ IsBuiltin name ∨ defs.any (·.1 = name) := by
+  simp [prog]
+
+@[simp]
+theorem def?_zero : prog.def? "0" = some defZero := by
+  simp [prog]; rw [Prog.def?_ofDefs (by simp)]; simp [defs, mainName]
+
+@[simp]
+theorem def?_one : prog.def? "1" = some defOne := by
+  simp [prog]; rw [Prog.def?_ofDefs (by simp)]; simp [defs, mainName]
+
+@[simp]
+theorem def?_not : prog.def? "not" = some defNot := by
+  simp [prog]; rw [Prog.def?_ofDefs (by simp)]; simp [defs, mainName]
+
+@[simp]
+theorem def?_bool : prog.def? "bool" = some defBool := by
+  simp [prog]; rw [Prog.def?_ofDefs (by simp)]; simp [defs, mainName]
+
+@[simp]
+theorem def?_add : prog.def? "add" = some defAdd := by
+  simp [prog]; rw [Prog.def?_ofDefs (by simp)]; simp [defs, mainName]
+
+@[simp]
+theorem def?_ite : prog.def? "ite" = some defIte := by
+  simp [prog]; rw [Prog.def?_ofDefs (by simp)]; simp [defs, mainName]
+
+-- #check 0 #exit
+
+@[simp]
+theorem wfDefs' : WFDefs' defs := by
+  use nodup_defs
+  · simp [defs]; decide
+  · simp [defs]
+  intro name d
+  rw [←prog]
+  simp [defs]
+  revert name d
+  simp
+  have h_zero : ∀ k, zero.WF prog k := λ _ => wf_zero # by simp
+  have h_one : ∀ k, one.WF prog k := λ _ => wf_one # by simp
+  apply and_of
+  · simp [exprZero, h_zero]
+  intro h_zero'
+  apply and_of
+  · simp [exprOne, h_zero]
+  intro h_one'
+  apply and_of
+  · simp [defNot, h_one]
+  intro h_not
+  apply and_of
+  · simp [defBool, isBuiltin_lit, defs, Prog.arity, Prog.def_eq_get!_def?]
+  intro h_bool
+  apply and_of
+  · simp [defAdd, exprAdd, isBuiltin_lit]
+    simp [defs, Prog.arity, Prog.def_eq_get!_def?, h_zero, h_one]
+  intro h_add
+  apply And.left (b := True)
+  apply and_of
+  · simp [defIte, exprIte, isBuiltin_lit]
+    simp [defs, Prog.arity, Prog.def_eq_get!_def?, h_zero, h_one]
+  intro h_ite
+  trivial
+
+-- #check 0 #exit
+
+@[instance, simp]
+theorem wf' : prog.WF' :=
+  wfDefs'.wf'
+
+@[simp]
+theorem union_fs : builtinFs ∪ .ofList fs = fsMap := rfl
+
+theorem builtin_not_name_of_mem_fs {name₁ name d} [H : BuiltinC name₁]
+(h : (name, d) ∈ fs) : name₁ ≠ name := by
+  replace h : name ∈ Map.ofList fs; simp; tauto
+  clear d; simp [fs] at h; revert name; simp
+  obtain ⟨⟨⟩, rfl⟩ := H <;> decide
+
+theorem get!_fsMap {name} : fsMap.get! name = match fs.find? (·.1 = name) with
+| .some p => p.2 | .none => builtinFs.get! name := by
+  split
+  · nm x p h; clear x
+    rcases p with ⟨name₁, d⟩
+    simp [List.find?_eq_some_iff_of_nodup] at h
+    rcases h with ⟨h₁, rfl⟩
+    unfold fsMap
+    rw [Map.get!_union_right # by simp [isBuiltin_iff, builtin_not_name_of_mem_fs h₁]]
+    rw [Map.get!_eq_get!_get?, Map.get?_ofList_of_nodup_and_mem (by simp) h₁]
+    rfl
+  · nm x h; clear x
+    simp at h ⊢
+    unfold fsMap
+    rw [Map.get!_union_left]
+    simp; grind
+
+@[simp]
+theorem not_builtin_mem_fs {name f} [H : BuiltinC name] : (name, f) ∉ fs := by
+  obtain ⟨b, rfl⟩ := H
+  suffices h : fs.map (·.1) |>.all (isBuiltin · = false)
+  · simp at h
+    intro h₁
+    specialize h _ _ h₁
+    have h₂ : IsBuiltin b.name; simp
+    rw [isBuiltin_iff_decide] at h₂
+    grind
+  unfold isBuiltin builtins; simp [fs]; decide
+
+@[simp]
+theorem get!_fsMap_builtin {name} [H : BuiltinC name] : fsMap.get! name = H.b.eval := by
+  rw [fsMap, Map.get!_union_left (by simp)]; simp
+
+@[simp]
+theorem get!_fsMap_zero : fsMap.get! "0" = fn 0 (λ _ => 0) := by
+  simp [get!_fsMap, fs, mainName]
+
+@[simp]
+theorem get!_fsMap_one : fsMap.get! "1" = fn 0 (λ _ => 1) := by
+  simp [get!_fsMap, fs, mainName]
+
+@[simp]
+theorem get!_fsMap_not : fsMap.get! "not" = fn 1 (λ xs => if xs[0]! = 0 then 1 else 0) := by
+  simp [get!_fsMap, fs, mainName]
+
+@[simp]
+theorem get!_fsMap_bool : fsMap.get! "bool" = fn 1 (λ xs => if xs[0]! = 0 then 0 else 1) := by
+  simp [get!_fsMap, fs, mainName]
+
+@[simp]
+theorem get!_fsMap_add : fsMap.get! "add" = fn 2 (λ xs => xs[0]! + xs[1]!) := by
+  simp [get!_fsMap, fs, mainName]
+
+@[simp]
+theorem get!_fsMap_ite : fsMap.get! "ite" = fn 3 (λ xs =>
+if xs[0]! = 0 then xs[2]! else xs[1]!) := by
+  simp [get!_fsMap, fs, mainName]
+
+-- #check 0 #exit
+
+@[simp]
+theorem eval_zero {xs} : zero.eval prog fsMap xs = 0 := by
+  simp [zero, fn]
+
+@[simp]
+theorem eval_one {xs} : one.eval prog fsMap xs = 1 := by
+  simp [one, fn]
+
+@[simp]
+theorem compatibleDefs : CompatibleDefs (.ofList defs) (.ofList fs) := by
+  use by simp [defs, fs, ExiVarC.exi_iff]
+  intro name d
+  rw [Prog.eq_ofDefs, ←prog]
+  intro h
+  rw [Map.get?_ofList_eq_some_iff (by simp)] at h
+  simp [defs] at h
+  revert name d
+  simp [Map.get?_ofList_eq_some_iff]
+  simp [fs, mainName]
+  apply and_of
+  · simp [exprId]
+  intro h_main
+  apply and_of
+  · simp [exprZero, fn]
+  intro h_zero
+  apply and_of
+  · simp [exprOne, fn]
+  intro h_one
+  apply and_of
+  · simp [defNot, fn]; grind
+  intro h_not
+  apply and_of
+  · simp [defBool, fn]
+  intro h_bool
+  apply and_of
+  · intro a b; simp [defAdd, exprAdd, fn]; grind
+  intro h_add
+  apply And.left (b := True)
+  apply and_of
+  · intro a b; simp [defIte, exprIte, fn]; grind
+  intro h_ite
+  trivial
+
+-- #check 0 #exit
+
+@[simp]
+theorem compatible : prog.Compatible fsMap :=
+  wfDefs'.compatible compatibleDefs
+
+theorem fs₁_get!_of {fs₁ name} (h : CompatibleDefs (.ofList defs) fs₁)
+(d : Def) (h₁ : (name, d) ∈ defs)
+(h₂ : ∀ f, (Map.ofList defs).get! name = d → (builtinFs ∪ fs₁).get! name = f →
+fs₁.get? name = some (fn d.arity (d.expr.eval prog (builtinFs ∪ fs₁))) →
+fs₁.get? name = some f → f = fn d.arity (d.expr.eval prog (builtinFs ∪ fs₁)) →
+fn d.arity f = Map.get! name (Map.ofList fs)) :
+(builtinFs ∪ fs₁).get! name = Map.get! name (Map.ofList fs) := by
+  have h₃ : (Map.ofList defs).get? name = d
+  · rwa [Map.get?_ofList_eq_some_iff (by simp)]
+  obtain ⟨f, h₄⟩ : ∃ f, fs₁.get? name = some f
+  · rw [←Map.mem_iff_get?_eq_some]
+    have h₄ := congrArg (name ∈ ·) h.keys_fs
+    simp at h₄
+    tauto
+  have h₅ : (builtinFs ∪ fs₁).get? name = some f
+  · rwa [Map.get?_union_right # by simp [wfDefs'.not_isBuiltin_of_mem h₁]]
+  have h₆ := h.get?_eq' h₃
+  simp [h₄] at h₆
+  rw [←Prog.ofDefs, ←prog] at h₆
+  rw [Map.get!_eq_get!_get?, h₅]; dsimp
+  rw [←h₂ f]; simp [h₆]
+  · exact Map.get!_ofList_of_nodup_and_mem (by simp) h₁
+  · simp [Map.get!_eq_get!_get?, h₅]
+  · simpa [h₄]
+  · exact h₄
+  · exact h₆
+
+@[simp]
+theorem get!_defs_main : (Map.ofList defs).get! mainName = ⟨1, exprId⟩ := by
+  simp [defs, Map.ofList_eq_foldl, Map.get!_insert, mainName]
+
+@[simp]
+theorem get!_defs_zero : (Map.ofList defs).get! "0" = defZero := by
+  simp [defs, Map.ofList_eq_foldl, Map.get!_insert, mainName]
+
+@[simp]
+theorem get!_defs_one : (Map.ofList defs).get! "1" = defOne := by
+  simp [defs, Map.ofList_eq_foldl, Map.get!_insert, mainName]
+
+@[simp]
+theorem get!_defs_not : (Map.ofList defs).get! "not" = defNot := by
+  simp [defs, Map.ofList_eq_foldl, Map.get!_insert, mainName]
+
+@[simp]
+theorem get!_defs_bool : (Map.ofList defs).get! "bool" = defBool := by
+  simp [defs, Map.ofList_eq_foldl, Map.get!_insert, mainName]
+
+@[simp]
+theorem get!_defs_add : (Map.ofList defs).get! "add" = defAdd := by
+  simp [defs, Map.ofList_eq_foldl, Map.get!_insert, mainName]
+
+@[simp]
+theorem get!_defs_ite : (Map.ofList defs).get! "ite" = defIte := by
+  simp [defs, Map.ofList_eq_foldl, Map.get!_insert, mainName]
+
+-- #check 0 #exit
+
+@[simp]
+theorem get!_fs_main : (Map.ofList fs).get! mainName = fn 1 (·[0]!) := by
+  simp [fs, Map.ofList_eq_foldl, Map.get!_insert, mainName]
+
+@[simp]
+theorem get!_fs_zero : (Map.ofList fs).get! "0" = fn 0 (λ _ => 0) := by
+  simp [fs, Map.ofList_eq_foldl, Map.get!_insert, mainName]
+
+@[simp]
+theorem get!_fs_one : (Map.ofList fs).get! "1" = fn 0 (λ _ => 1) := by
+  simp [fs, Map.ofList_eq_foldl, Map.get!_insert, mainName]
+
+@[simp]
+theorem get!_fs_not : (Map.ofList fs).get! "not" =
+fn 1 (λ xs => if xs[0]! = 0 then 1 else 0) := by
+  simp [fs, Map.ofList_eq_foldl, Map.get!_insert, mainName]
+
+@[simp]
+theorem get!_fs_bool : (Map.ofList fs).get! "bool" =
+fn 1 (λ xs => if xs[0]! = 0 then 0 else 1) := by
+  simp [fs, Map.ofList_eq_foldl, Map.get!_insert, mainName]
+
+@[simp]
+theorem get!_fs_add : (Map.ofList fs).get! "add" =
+fn 2 (λ xs => xs[0]! + xs[1]!) := by
+  simp [fs, Map.ofList_eq_foldl, Map.get!_insert, mainName]
+
+@[simp]
+theorem get!_fs_ite : (Map.ofList fs).get! "ite" =
+fn 3 (λ xs => if xs[0]! = 0 then xs[2]! else xs[1]!) := by
+  simp [fs, Map.ofList_eq_foldl, Map.get!_insert, mainName]
+
+-- #check 0 #exit
+
+theorem fs₁_get?_builtin {fs₁ name} [H : BuiltinC name]
+(h : CompatibleDefs (.ofList defs) fs₁) : (builtinFs ∪ fs₁).get? name = some H.b.eval := by
+  simp [h.get?_builtin]
+
+theorem fs₁_get?_main {fs₁} (h : CompatibleDefs (.ofList defs) fs₁) :
+fs₁.get? mainName = some (fn 1 # exprId.eval prog (builtinFs ∪ fs₁)) := by
+  simp [(@h.eval_eq) mainName defId (by simp [defs])]; rw [←Prog.ofDefs, ←prog]; simp
+
+theorem fs₁_get?_zero {fs₁} (h : CompatibleDefs (.ofList defs) fs₁) :
+fs₁.get? "0" = some (fn 0 # exprZero.eval prog (builtinFs ∪ fs₁)) := by
+  simp [(@h.eval_eq) "0" defZero (by simp [defs])]; rw [←Prog.ofDefs, ←prog]
+
+theorem fs₁_get?_one {fs₁} (h : CompatibleDefs (.ofList defs) fs₁) :
+fs₁.get? "1" = some (fn 0 # exprOne.eval prog (builtinFs ∪ fs₁)) := by
+  simp [(@h.eval_eq) "1" defOne (by simp [defs])]; rw [←Prog.ofDefs, ←prog]
+
+theorem fs₁_get?_not {fs₁} (h : CompatibleDefs (.ofList defs) fs₁) :
+fs₁.get? "not" = some (fn 1 # defNot.expr.eval prog (builtinFs ∪ fs₁)) := by
+  simp [(@h.eval_eq) "not" defNot (by simp [defs])]; rw [←Prog.ofDefs, ←prog]; simp
+
+theorem fs₁_get?_bool {fs₁} (h : CompatibleDefs (.ofList defs) fs₁) :
+fs₁.get? "bool" = some (fn 1 # defBool.expr.eval prog (builtinFs ∪ fs₁)) := by
+  simp [(@h.eval_eq) "bool" defBool (by simp [defs])]; rw [←Prog.ofDefs, ←prog]; simp
+
+theorem fs₁_get?_add {fs₁} (h : CompatibleDefs (.ofList defs) fs₁) :
+fs₁.get? "add" = some (fn 2 # defAdd.expr.eval prog (builtinFs ∪ fs₁)) := by
+  simp [(@h.eval_eq) "add" defAdd (by simp [defs])]; rw [←Prog.ofDefs, ←prog]; simp
+
+theorem fs₁_get?_ite {fs₁} (h : CompatibleDefs (.ofList defs) fs₁) :
+fs₁.get? "ite" = some (fn 3 # defIte.expr.eval prog (builtinFs ∪ fs₁)) := by
+  simp [(@h.eval_eq) "ite" defIte (by simp [defs])]; rw [←Prog.ofDefs, ←prog]; simp
+
+-- #check 0 #exit
+
+theorem fs₁_get!_builtin {fs₁ name} [H : BuiltinC name]
+(h : CompatibleDefs (.ofList defs) fs₁) : (builtinFs ∪ fs₁).get! name = H.b.eval := by
+  rw [Map.get!_union_left]; simp
+  intro h₁
+  have h₂ := congrArg (H.b.name ∈ ·) h.keys_fs
+  simp [h₁] at h₂
+  choose d h₂ using h₂
+  have h₃ := wfDefs'.not_isBuiltin_of_mem h₂
+  simp at h₃
+
+theorem fs₁_get!_main {fs₁} (h : CompatibleDefs (.ofList defs) fs₁) :
+(builtinFs ∪ fs₁).get! mainName = (Map.ofList fs).get! mainName := by
+  rw [Map.get!_union_right # by simp]
+  rw [Map.get!_eq_get!_get?, fs₁_get?_main h]; simp
+  simp [exprId]
+
+theorem fs₁_get!_zero {fs₁} (h : CompatibleDefs (.ofList defs) fs₁) :
+(builtinFs ∪ fs₁).get! "0" = (Map.ofList fs).get! "0" := by
+  rw [Map.get!_union_right # by simp; decide]
+  rw [Map.get!_eq_get!_get?, fs₁_get?_zero h]; simp
+  simp [exprZero, fs₁_get!_builtin h, fn]
+
+theorem fs₁_zero {fs₁ xs} (h : CompatibleDefs (.ofList defs) fs₁) :
+zero.eval prog (builtinFs ∪ fs₁) xs = 0 := by
+  simp [zero, fs₁_get!_zero h, fn]
+
+theorem fs₁_get!_one {fs₁} (h : CompatibleDefs (.ofList defs) fs₁) :
+(builtinFs ∪ fs₁).get! "1" = (Map.ofList fs).get! "1" := by
+  rw [Map.get!_union_right # by simp; decide]
+  rw [Map.get!_eq_get!_get?, fs₁_get?_one h]; simp
+  simp [exprOne, fs₁_get!_builtin h, fn, fs₁_zero h]
+
+theorem fs₁_one {fs₁ xs} (h : CompatibleDefs (.ofList defs) fs₁) :
+one.eval prog (builtinFs ∪ fs₁) xs = 1 := by
+  simp [one, fs₁_get!_one h, fn]
+
+theorem fs₁_get!_not {fs₁} (h : CompatibleDefs (.ofList defs) fs₁) :
+(builtinFs ∪ fs₁).get! "not" = (Map.ofList fs).get! "not" := by
+  rw [Map.get!_union_right # by simp; decide]
+  rw [Map.get!_eq_get!_get?, fs₁_get?_not h]; simp
+  simp [defNot]; intro n; simp [fs₁_get!_builtin h, fn, fs₁_one h]; grind
+
+theorem fs₁_get!_bool {fs₁} (h : CompatibleDefs (.ofList defs) fs₁) :
+(builtinFs ∪ fs₁).get! "bool" = (Map.ofList fs).get! "bool" := by
+  rw [Map.get!_union_right # by simp; decide]
+  rw [Map.get!_eq_get!_get?, fs₁_get?_bool h]; simp
+  simp [defBool]; intro n; simp [fn, fs₁_get!_not h]
+
+theorem exprAdd_aux (f : ℕ → ℕ → ℕ) (h : ∀ x y, f x y = f (x - 1) (y - 1) + 2 -
+(if x = 0 then 1 else 0) - (if y = 0 then 1 else 0) - f 0 0) : f = (· + ·) := by
+  ext x y
+  have h₁ : f 0 0 = 0
+  · specialize h 0 0
+    simpa using h
+  induction x generalizing y
+  · specialize h 0
+    simp at h
+    induction y
+    · specialize h 0
+      simpa using h
+    nm y ih
+    specialize h (y + 1)
+    simp_all
+  nm x ih
+  specialize h (x + 1) y
+  simp_all
+  specialize ih (y + 1)
+  grind
+
+theorem fs₁_get!_add {fs₁} (h : CompatibleDefs (.ofList defs) fs₁) :
+(builtinFs ∪ fs₁).get! "add" = (Map.ofList fs).get! "add" := by
+  apply fs₁_get!_of h defAdd (by simp [defs])
+  intro f h₁ h₂ h₃ h₄ h₅
+  simp [h₄, defAdd, exprAdd, funext_iff, fn, fs₁_get!_builtin h, h₂,
+    fs₁_zero h, fs₁_one h, fs₁_get!_not h] at h₃
+  have h₆ := forall_imp_of_forall (λ (xs : List _) => xs.length = 2) h₃
+  simp at h₆; clear h₁ h₂ h₃ h₄ h₅; rename' h₆ => h₁
+  have h₂ := exprAdd_aux (f [·, ·]); specialize h₂ _
+  on_goal 2 => simpa [funext_iff] using h₂;; clear h₂; exact h₁
+
+theorem exprIte_aux (f : ℕ → ℕ → ℕ → ℕ) (h : ∀ a b c, f a b c =
+f a (b - 1) (c - 1) + 1 - ((if a = 0 then 0 else 1) - b) -
+((if a = 0 then 1 else 0) - c) - f a 0 0) :
+f = λ a b c => if a = 0 then c else b := by
+  classical
+  ext a b c
+  simp [Nat.ite_eq_ofProp, Nat.ite_eq_ofProp'] at h
+  have h₁ : ∀ a, f a 0 0 = 0
+  · clear a b c; intro a; rw [h]; simp
+  simp [h₁] at h
+  by_cases ha : a = 0 <;> simp [ha]
+  · clear! a
+    induction c generalizing b
+    · induction b
+      · rw [h₁]
+      nm b ih
+      rw [h]
+      simpa
+    nm c ih
+    rw [h]
+    simp [ih]
+  · induction c generalizing b
+    · induction b
+      · rw [h₁]
+      nm b ih
+      rw [h]
+      simpa [ha]
+    nm c ih
+    rw [h]
+    simp [ha, ih]
+    cases b <;> simp
+
+theorem fs₁_get!_ite {fs₁} (h : CompatibleDefs (.ofList defs) fs₁) :
+(builtinFs ∪ fs₁).get! "ite" = (Map.ofList fs).get! "ite" := by
+  apply fs₁_get!_of h defIte (by simp [defs])
+  intro f h₁ h₂ h₃ h₄ h₅
+  simp [h₄, defIte, exprIte, funext_iff, fn, fs₁_get!_builtin h, h₂,
+    fs₁_zero h, fs₁_one h, fs₁_get!_not h, fs₁_get!_bool h] at h₃
+  have h₆ := forall_imp_of_forall (λ (xs : List _) => xs.length = 3) h₃
+  simp at h₆; clear h₁ h₂ h₃ h₄ h₅; rename' h₆ => h₁
+  have h₂ := exprIte_aux (f [·, ·, ·]); specialize h₂ _
+  on_goal 2 => simpa [funext_iff] using h₂;; clear h₂; exact h₁
+
+-- #check 0 #exit
+
+@[instance, simp]
+theorem wf_prog : prog.WF := by
+  apply wfDefs'.wf; use .ofList fs, compatibleDefs
+  intro fs₁ h name d f h₂ h₃
+  have h₅ := h.eval_eq h₂ |>.symm
+  rw [←Prog.ofDefs, ←prog] at h₅
+  simp [h₃] at h₅
+  subst h₅
+  simp [funext_iff]
+  intro xs
+  simp [defs] at h₂
+  revert h₃
+  revert name d h₂
+  simp [eq_comm (b := Expr.eval _ _ _ _)]
+  simp [fs₁_get?_main h, fs₁_get?_zero h, fs₁_get?_one h]
+  revert xs
+  simp only [imp_comm_left (b := List.length _ = _)]
+  intro xs; apply and_of
+  · simp [exprId]
+  rintro -; revert xs
+  intro xs; apply and_of
+  · simp [exprZero, fs₁_get!_builtin h, fn]
+  rintro -; revert xs
+  intro xs; apply and_of
+  · simp [exprOne, fs₁_get!_builtin h, fn, fs₁_zero h]
+  rintro -; revert xs
+  apply imp_fs_and_of # fs₁_get?_not h
+  · simp; intro n; simp [defNot, fs₁_get!_builtin h, fs₁_one h, fn]; grind
+  intro h_not
+  apply imp_fs_and_of # fs₁_get?_bool h
+  · simp; intro n; simp [defBool, h_not, fn]
+  intro h_bool
+  apply imp_fs_and_of # fs₁_get?_add h
+  · simp; intro n m
+    simp [defAdd, exprAdd, fs₁_get!_builtin h, fn, fs₁_get!_add h,
+      fs₁_one h, fs₁_zero h, h_not]; grind
+  intro h_add
+  apply forall_and_true
+  apply imp_fs_and_of # fs₁_get?_ite h
+  · simp; intro a b c
+    simp [defIte, exprIte, fs₁_get!_builtin h, fn, fs₁_get!_ite h,
+      fs₁_zero h, fs₁_one h, h_bool, h_not]; grind
+  intro h_ite
+  simp
+    
+-- #check 0 #exit
+
+instance : ProgInfo prog where
+  name := "Prog₁"
+  defNames := ["main", "0", "1", "not", "bool", "add", "ite"]
+  has_model := true
+  has_unique_model := true
+  h_defNames := by
+    dsimp [prog, Prog.ofDefs]
+    rw [Map.keys_union # by simp [isBuiltin_iff, Builtin.all, defs, mainName, succName, subName]]
+    simp only [builtinDefs, List.map_map, Function.comp_def, nodup_map_name_builtins,
+      Map.keys_ofList, nodup_defs, List.mergeSort_perm_iff, List.append_mergeSort_perm,
+      List.mergeSort_append_perm, List.perm_append_left_iff]
+    simp [defs]; decide
+  h_wf' := by simp
+  h_has_model := by
+    simp [Prog.HasModel]; use prog.fs; apply τ_spec; use builtinFs ∪ .ofList fs; simp
+  h_has_unique_model := by have := wf_prog.exiu_compatible; simp [Prog.HasUniqueModel]; tauto
