Projects/Esolangs/Cornucopia/Programs.lean
@@ -2,4 +2,5 @@ import Projects.Esolangs.Cornucopia.Programs.Id
 import Projects.Esolangs.Cornucopia.Programs.Loop
 import Projects.Esolangs.Cornucopia.Programs.LoopSucc1
 import Projects.Esolangs.Cornucopia.Programs.LoopSucc2
+import Projects.Esolangs.Cornucopia.Programs.OneAlt1
 import Projects.Esolangs.Cornucopia.Programs.Prog1
