Projects/Esolangs/Cornucopia/Programs/Common.lean
@@ -1,0 +1,100 @@
+import Projects.Esolangs.Cornucopia.Basic
+
+attribute [-simp] List.getElem!_eq_getElem?_getD
+
+namespace Esolangs.Cornucopia
+
+-----
+
+@[simp]
+def Expr.const (name : String) : Expr :=
+  .call name []
+
+def exprId : Expr :=
+  .arg 0
+
+@[simp]
+def defId : Def :=
+  ⟨1, exprId⟩
+
+def exprLoop (name : String) : Expr :=
+  .call name [.arg 0]
+
+@[simp]
+def defLoop (name : String) : Def :=
+  ⟨1, exprLoop name⟩
+
+def exprLoopSucc₁ (name : String) : Expr :=
+  .call succName [.call name [.arg 0]]
+
+@[simp]
+def defLoopSucc₁ (name : String) : Def :=
+  ⟨1, exprLoopSucc₁ name⟩
+
+def exprLoopSucc₂ (name : String) : Expr :=
+  .call name [.call succName [.arg 0]]
+
+@[simp]
+def defLoopSucc₂ (name : String) : Def :=
+  ⟨1, exprLoopSucc₂ name⟩
+
+def zero : Expr :=
+  .const "0"
+
+def exprZero : Expr :=
+  .call subName [zero, zero]
+
+@[simp]
+def defZero : Def :=
+  ⟨0, exprZero⟩
+
+def one : Expr :=
+  .const "1"
+
+def exprOne : Expr :=
+  .call succName [zero]
+
+@[simp]
+def defOne : Def :=
+  ⟨0, exprOne⟩
+
+-- #check 0 #exit
+
+-----
+
+@[simp] theorem arity_defId : defId.arity = 1 := rfl
+@[simp] theorem expr_defId : defId.expr = exprId := rfl
+
+@[simp]
+theorem wf_exprId {prog} : exprId.WF prog 1 := by
+  simp [exprId]
+
+theorem wf_exprLoop {prog name}
+(h : prog.def? name = some (defLoop name)) : (exprLoop name).WF prog 1 := by
+  simp [exprLoop, Prog.HasDef, Map.mem_of_get?_eq_some h, Prog.arity, Prog.def_eq_get!_def?, h]
+
+theorem wf_exprLoopSucc₁ {prog : Prog} {name} [H : prog.WFBuiltins]
+(h : prog.def? name = some (defLoopSucc₁ name)) : (exprLoopSucc₁ name).WF prog 1 := by
+  simp [exprLoopSucc₁, prog.hasDef_of_def? h, prog.arity_of_def? h]
+
+theorem wf_exprLoopSucc₂ {prog : Prog} {name} [H : prog.WFBuiltins]
+(h : prog.def? name = some (defLoopSucc₂ name)) : (exprLoopSucc₂ name).WF prog 1 := by
+  simp [exprLoopSucc₂, prog.hasDef_of_def? h, prog.arity_of_def? h]
+
+theorem Expr.wf_const {prog : Prog} {name d k}
+(h₁ : prog.def? name = some d) (h₂ : d.arity = 0) : (Expr.const name).WF prog k := by
+  simp [Prog.hasDef_of_def? h₁, Prog.arity_of_def? h₁, h₂]
+
+theorem wf_zero {prog : Prog} {k} (h : prog.def? "0" = some defZero) : zero.WF prog k :=
+  Expr.wf_const h rfl
+
+theorem wf_one {prog : Prog} {k} (h : prog.def? "1" = some defOne) : one.WF prog k :=
+  Expr.wf_const h rfl
+
+theorem wf_exprZero {prog : Prog} [H : prog.WFBuiltins] {k}
+(h : prog.def? "0" = some defZero) : exprZero.WF prog k := by
+  simp [exprZero, wf_zero h]
+
+theorem wf_exprOne {prog : Prog} [H : prog.WFBuiltins] {k}
+(h : prog.def? "0" = some defZero) : exprOne.WF prog k := by
+  simp [exprOne, wf_zero h]
