Projects/Esolangs/Cornucopia/Programs/OneAlt1.lean
@@ -1,0 +1,271 @@
+import Projects.Esolangs.Cornucopia.Programs.Common
+
+attribute [-simp] List.getElem!_eq_getElem?_getD
+
+namespace Esolangs.Cornucopia.OneAlt₁
+
+def exprOneAlt : Expr :=
+  .call subName
+  [ .call succName [.call "1" []]
+  , .call "1" []
+  ]
+
+def defOneAlt : Def :=
+  ⟨0, exprOneAlt⟩
+
+def defMain : Def :=
+  ⟨1, .call "1" []⟩
+
+def defs : List (String × Def) :=
+  [ (mainName, defMain)
+  , ("1", defOneAlt)
+  ]
+
+def fs : List (String × (List ℕ → ℕ)) :=
+  [ (mainName, fn 1 λ _ => 1)
+  , ("1", fn 0 λ _ => 1)
+  ]
+
+def fsMap : Map String (List ℕ → ℕ) :=
+  builtinFs ∪ .ofList fs
+
+def prog : Prog :=
+  .ofDefs defs
+
+-- #check 0 #exit
+
+-----
+
+@[simp]
+theorem nodup_defs : defs.map (·.1) |>.Nodup := by
+  decide
+
+@[simp]
+theorem nodup_fs : fs.map (·.1) |>.Nodup := by
+  decide
+
+@[instance, simp]
+theorem wfBuiltins_prog : prog.WFBuiltins := by
+  apply Prog.wfBuiltins_ofDefs; decide
+
+@[simp] theorem arity_oneAlt : defOneAlt.arity = 0 := rfl
+
+-- #check 0 #exit
+
+@[simp]
+theorem hasDef_prog_iff {name} : prog.HasDef name ↔ IsBuiltin name ∨ defs.any (·.1 = name) := by
+  simp [prog]
+
+@[simp]
+theorem def?_oneAlt : prog.def? "1" = some defOneAlt := by
+  simp [prog]; rw [Prog.def?_ofDefs (by simp)]; simp [defs, mainName]
+
+-- #check 0 #exit
+
+@[simp]
+theorem wfDefs' : WFDefs' defs := by
+  use nodup_defs
+  · simp [defs]; decide
+  · simp [defs, defMain]
+  intro name d
+  rw [←prog]
+  simp [defs]
+  revert name d
+  simp [defOneAlt, exprOneAlt, defs, Prog.arity, Prog.def_eq_get!_def?, defMain]
+
+-- #check 0 #exit
+
+@[instance, simp]
+theorem wf' : prog.WF' :=
+  wfDefs'.wf'
+
+@[simp]
+theorem union_fs : builtinFs ∪ .ofList fs = fsMap := rfl
+
+theorem builtin_not_name_of_mem_fs {name₁ name d} [H : BuiltinC name₁]
+(h : (name, d) ∈ fs) : name₁ ≠ name := by
+  replace h : name ∈ Map.ofList fs; simp; tauto
+  clear d; simp [fs] at h; revert name; simp
+  obtain ⟨⟨⟩, rfl⟩ := H <;> decide
+
+theorem get!_fsMap {name} : fsMap.get! name = match fs.find? (·.1 = name) with
+| .some p => p.2 | .none => builtinFs.get! name := by
+  split
+  · nm x p h; clear x
+    rcases p with ⟨name₁, d⟩
+    simp [List.find?_eq_some_iff_of_nodup] at h
+    rcases h with ⟨h₁, rfl⟩
+    unfold fsMap
+    rw [Map.get!_union_right # by simp [isBuiltin_iff, builtin_not_name_of_mem_fs h₁]]
+    rw [Map.get!_eq_get!_get?, Map.get?_ofList_of_nodup_and_mem (by simp) h₁]
+    rfl
+  · nm x h; clear x
+    simp at h ⊢
+    unfold fsMap
+    rw [Map.get!_union_left]
+    simp; grind
+
+@[simp]
+theorem not_builtin_mem_fs {name f} [H : BuiltinC name] : (name, f) ∉ fs := by
+  obtain ⟨b, rfl⟩ := H
+  suffices h : fs.map (·.1) |>.all (isBuiltin · = false)
+  · simp at h
+    intro h₁
+    specialize h _ _ h₁
+    have h₂ : IsBuiltin b.name; simp
+    rw [isBuiltin_iff_decide] at h₂
+    grind
+  unfold isBuiltin builtins; simp [fs]; decide
+
+@[simp]
+theorem get!_fsMap_builtin {name} [H : BuiltinC name] : fsMap.get! name = H.b.eval := by
+  rw [fsMap, Map.get!_union_left (by simp)]; simp
+
+@[simp]
+theorem get!_fsMap_oneAlt : fsMap.get! "1" = fn 0 (λ _ => 1) := by
+  simp [get!_fsMap, fs, mainName]
+
+-- #check 0 #exit
+
+@[simp]
+theorem compatibleDefs : CompatibleDefs (.ofList defs) (.ofList fs) := by
+  use by simp [defs, fs, ExiVarC.exi_iff]
+  intro name d
+  rw [Prog.eq_ofDefs, ←prog]
+  intro h
+  rw [Map.get?_ofList_eq_some_iff (by simp)] at h
+  simp [defs] at h
+  revert name d
+  simp [Map.get?_ofList_eq_some_iff]
+  simp [fs, mainName]
+  simp [defOneAlt, exprOneAlt, defMain, fn]
+
+-- #check 0 #exit
+
+@[simp]
+theorem compatible : prog.Compatible fsMap :=
+  wfDefs'.compatible compatibleDefs
+
+theorem fs₁_get!_of {fs₁ name} (h : CompatibleDefs (.ofList defs) fs₁)
+(d : Def) (h₁ : (name, d) ∈ defs)
+(h₂ : ∀ f, (Map.ofList defs).get! name = d → (builtinFs ∪ fs₁).get! name = f →
+fs₁.get? name = some (fn d.arity (d.expr.eval prog (builtinFs ∪ fs₁))) →
+fs₁.get? name = some f → f = fn d.arity (d.expr.eval prog (builtinFs ∪ fs₁)) →
+fn d.arity f = Map.get! name (Map.ofList fs)) :
+(builtinFs ∪ fs₁).get! name = Map.get! name (Map.ofList fs) := by
+  have h₃ : (Map.ofList defs).get? name = d
+  · rwa [Map.get?_ofList_eq_some_iff (by simp)]
+  obtain ⟨f, h₄⟩ : ∃ f, fs₁.get? name = some f
+  · rw [←Map.mem_iff_get?_eq_some]
+    have h₄ := congrArg (name ∈ ·) h.keys_fs
+    simp at h₄
+    tauto
+  have h₅ : (builtinFs ∪ fs₁).get? name = some f
+  · rwa [Map.get?_union_right # by simp [wfDefs'.not_isBuiltin_of_mem h₁]]
+  have h₆ := h.get?_eq' h₃
+  simp [h₄] at h₆
+  rw [←Prog.ofDefs, ←prog] at h₆
+  rw [Map.get!_eq_get!_get?, h₅]; dsimp
+  rw [←h₂ f]; simp [h₆]
+  · exact Map.get!_ofList_of_nodup_and_mem (by simp) h₁
+  · simp [Map.get!_eq_get!_get?, h₅]
+  · simpa [h₄]
+  · exact h₄
+  · exact h₆
+
+@[simp]
+theorem get!_defs_main : (Map.ofList defs).get! mainName = defMain := by
+  simp [defs, Map.ofList_eq_foldl, Map.get!_insert, mainName]
+
+@[simp]
+theorem get!_defs_oneAlt : (Map.ofList defs).get! "1" = defOneAlt := by
+  simp [defs, Map.ofList_eq_foldl, Map.get!_insert, mainName]
+
+-- #check 0 #exit
+
+@[simp]
+theorem get!_fs_main : (Map.ofList fs).get! mainName = fn 1 (λ _ => 1) := by
+  simp [fs, Map.ofList_eq_foldl, Map.get!_insert, mainName]
+
+@[simp]
+theorem get!_fs_oneAlt : (Map.ofList fs).get! "1" = fn 0 (λ _ => 1) := by
+  simp [fs, Map.ofList_eq_foldl, Map.get!_insert, mainName]
+
+-- #check 0 #exit
+
+theorem fs₁_get?_builtin {fs₁ name} [H : BuiltinC name]
+(h : CompatibleDefs (.ofList defs) fs₁) : (builtinFs ∪ fs₁).get? name = some H.b.eval := by
+  simp [h.get?_builtin]
+
+theorem fs₁_get?_main {fs₁} (h : CompatibleDefs (.ofList defs) fs₁) :
+fs₁.get? mainName = some (fn 1 # defMain.expr.eval prog (builtinFs ∪ fs₁)) := by
+  simp [(@h.eval_eq) mainName defMain (by simp [defs])]; rw [←Prog.ofDefs, ←prog]; rfl
+
+theorem fs₁_get?_oneAlt {fs₁} (h : CompatibleDefs (.ofList defs) fs₁) :
+fs₁.get? "1" = some (fn 0 # exprOneAlt.eval prog (builtinFs ∪ fs₁)) := by
+  simp [(@h.eval_eq) "1" defOneAlt (by simp [defs])]; rw [←Prog.ofDefs, ←prog]; rfl
+
+-- #check 0 #exit
+
+theorem fs₁_get!_builtin {fs₁ name} [H : BuiltinC name]
+(h : CompatibleDefs (.ofList defs) fs₁) : (builtinFs ∪ fs₁).get! name = H.b.eval := by
+  rw [Map.get!_union_left]; simp
+  intro h₁
+  have h₂ := congrArg (H.b.name ∈ ·) h.keys_fs
+  simp [h₁] at h₂
+  choose d h₂ using h₂
+  have h₃ := wfDefs'.not_isBuiltin_of_mem h₂
+  simp at h₃
+
+theorem fs₁_get!_oneAlt {fs₁} (h : CompatibleDefs (.ofList defs) fs₁) :
+(builtinFs ∪ fs₁).get! "1" = (Map.ofList fs).get! "1" := by
+  apply fs₁_get!_of h defOneAlt (by simp [defs])
+  intro f h₁ h₂ h₃ h₄ h₅
+  simp [h₂, h₄, fn, funext_iff, defOneAlt, exprOneAlt, fs₁_get!_builtin h, fn] at h₃
+  have h₆ := forall_imp_of_forall (λ (xs : List _) => xs.length = 0) h₃
+  simp at h₆; clear h₁ h₂ h₃ h₄ h₅; rename' h₆ => h₁
+  ext xs; simp [fn]; grind
+
+theorem fs₁_get!_main {fs₁} (h : CompatibleDefs (.ofList defs) fs₁) :
+(builtinFs ∪ fs₁).get! mainName = (Map.ofList fs).get! mainName := by
+  rw [Map.get!_union_right # by simp]
+  rw [Map.get!_eq_get!_get?, fs₁_get?_main h]; simp
+  simp [defMain, fs₁_get!_oneAlt h, fn]
+
+-- #check 0 #exit
+
+@[instance, simp]
+theorem wf_prog : prog.WF := by
+  apply wfDefs'.wf; use .ofList fs, compatibleDefs
+  intro fs₁ h name d f h₂ h₃
+  have h₅ := h.eval_eq h₂ |>.symm
+  rw [←Prog.ofDefs, ←prog] at h₅
+  simp [h₃] at h₅
+  subst h₅
+  simp [funext_iff]
+  intro xs
+  simp [defs] at h₂
+  revert h₃
+  revert name d h₂
+  revert xs
+  simp [fs₁_get?_main h, fn, defMain, fs₁_get?_oneAlt h, fs₁_get!_oneAlt h,
+    exprOneAlt, fs₁_get!_builtin h]
+    
+-- #check 0 #exit
+
+instance : ProgInfo prog where
+  name := "OneAlt₁"
+  defNames := ["main", "1"]
+  has_model := true
+  has_unique_model := true
+  h_defNames := by
+    dsimp [prog, Prog.ofDefs]
+    rw [Map.keys_union # by simp [isBuiltin_iff, Builtin.all, defs, mainName, succName, subName]]
+    simp only [builtinDefs, List.map_map, Function.comp_def, nodup_map_name_builtins,
+      Map.keys_ofList, nodup_defs, List.mergeSort_perm_iff, List.append_mergeSort_perm,
+      List.mergeSort_append_perm, List.perm_append_left_iff]
+    simp [defs]; decide
+  h_wf' := by simp
+  h_has_model := by
+    simp [Prog.HasModel]; use prog.fs; apply τ_spec; use builtinFs ∪ .ofList fs; simp
+  h_has_unique_model := by have := wf_prog.exiu_compatible; simp [Prog.HasUniqueModel]; tauto
