Projects/Expr/Basic.lean
@@ -1,0 +1,339 @@
+import Projects.Expr.Defs
+
+section logic
+
+variable {α β γ : Type*}
+
+-- #check 0 #exit
+
+end logic
+
+namespace List
+
+variable {α β γ : Type*}
+variable {xs ys zs : List α}
+
+def wfLex [LT α] (xs ys : List α) : Prop :=
+  match compare xs.length ys.length with
+  | .lt => True
+  | .gt => False
+  | .eq => xs < ys
+
+theorem length_le_of_wfLex [ha : LT α] (h : wfLex xs ys) : xs.length ≤ ys.length := by
+  grind [wfLex]
+
+-- #check 0 #exit
+
+attribute [-instance] instLinearOrderOfDecidable_projects
+
+-- theorem wf_wfLex [H : WellFoundedRelation α] : WellFounded (wfLex (α := α)) := by
+--   classical
+--   constructor
+--   intro xs
+--   
+--   by_cases ha : IsEmpty α
+--   ·
+--     constructor
+--     intro ys h
+--     simp [wfLex, eq_nil_of_isEmpty] at h
+--     
+--   simp at ha
+--   
+--   generalize hn : xs.length = n
+--   induction n using Nat.strong_induction_on generalizing xs
+--   nm n ih
+--   
+--   cases n
+--   ·
+--     simp at hn
+--     constructor
+--     simp [wfLex, hn]
+--     grind
+--   nm n
+--   simp at ih
+--   
+--   rw [length_eq_succ_iff_append] at hn
+--   obtain ⟨x, xs, ys, rfl, rfl⟩ := hn
+--   
+--   -- by_contra! h₀
+--   -- have h₁ : ∀ x, ∀ y < x, ∀ (xs ys : List α), (∀ m ≤ xs.length + ys.length,
+--   --   ∀ (xs : List α), xs.length = m → Acc wfLex xs) → Acc wfLex (xs ++ y :: ys)
+--   -- ·
+--   --   contrapose! h₀
+--   --   choose x' y hy' xs' ys' h₂ h₃ using h₀
+--   --   have h₁ : ∀ x, Acc (λ a b => a < b) x := H.2.1
+--   
+--   obtain ⟨m, hm⟩ := hv λ (a b : α) => if Relation.TransGen H.rel a b then b else a
+--   letI : Max α := ⟨m⟩
+--   
+--   have h₁ : ∀ x, Acc (λ a b => a < b) x := H.2.1
+--   conv at h₁ => right; rw [←acc_transGen_iff]
+--   generalize hy : (xs ++ x :: ys).max! = y
+--   replace hy := le_of_eq hy
+--   specialize h₁ y
+--   
+--   induction h₁ generalizing x xs ys
+--   clear y
+--   nm y h₁ ih₁
+--   
+--   -- clear x
+--   -- nm x hx ih₁
+--   
+--   constructor
+--   intro zs h₂
+--   
+--   have h₃ := length_le_of_wfLex h₂
+--   rw [Nat.le_iff_lt_or_eq] at h₃
+--   rcases h₃ with h₃ | h₃; grind
+--   simp at h₃
+--   
+--   -- replace h₂ : ∃ z zs₁ zs₂, zs = zs₁ ++ z :: zs₂ ∧
+--   --   zs₁.length = xs.length ∧ zs₂.length = ys.length
+--   -- ·
+--   --   use zs[xs.length]!, zs.take xs.length, zs.drop (xs.length + 1)
+--   --   simp
+--   --   rw [List.getElem?_eq_getElem (by grind)]
+--   --   simp
+--   --   grind
+--   -- 
+--   -- obtain ⟨z, zs₁, zs₂, rfl, h₂, h₃⟩ := h₂
+--   
+--   simp [wfLex, h₃] at h₂
+--   rw [List.lt_iff_exists] at h₂
+--   simp [h₃] at h₂
+--   choose i h₂ h₄ h₅ using h₂
+--   
+--   obtain ⟨z, zs₁, zs₂, rfl, rfl⟩ := zs.exi_append_cons i (by omega)
+--   simp at h₅
+--   
+--   apply ih₁ z
+--   ·
+--     -- suffices : y ≤ (xs ++ x :: ys)[zs₁.length]; linarith
+--     -- apply h₅.trans_eq
+--     
+--     -- have H₁ : Relation.TransGen (· < ·) ((xs ++ x :: ys)[zs₁.length]'(by grind)) y
+--     -- ·
+--     --   exact?
+--     
+--     apply Relation.TransGen.lt_of_lt_of_le ((xs ++ x :: ys)[zs₁.length]'(by grind))
+--     ·
+--       constructor; exact h₅
+--     
+--     rw [or_iff_not_imp_left]
+--     intro h₆
+--     
+--     apply Relation.TransGen.lt_of_lt_of_le (xs ++ x :: ys).max!
+--     rotate_left
+--     ·
+--       rw [le_iff_eq_or_lt] at hy
+--       rcases hy with hy | hy
+--       ·
+--         exact .inl hy
+--       right
+--       
+--       constructor
+--       convert hy
+--     
+--     suffices : (xs ++ x :: ys)[zs₁.length]'(by grind) ≤ (xs ++ x :: ys).max!
+--     ·
+
+-- #check 0 #exit
+
+-- instance {α : Type} [H : WellFoundedRelation α] : WellFoundedRelation (List α) where
+--   rel := wfLex
+--   wf := wf_wfLex
+
+-- #check 0 #exit
+
+end List
+
+namespace Expr
+
+variable {a b c d e : Expr}
+
+@[simp] theorem isNil_nil : nil.isNil := trivial
+@[simp] theorem not_isNil_pair : ¬(pair a b).isNil := by simp [isNil]
+@[simp] theorem not_isPair_nil : ¬nil := by simp [isPair]
+@[simp] theorem isPair_pair : pair a b := trivial
+@[simp] theorem fst_nil : nil.fst = nil := rfl
+@[simp] theorem snd_nil : nil.snd = nil := rfl
+@[simp] theorem fst_pair : (pair a b).fst = a := rfl
+@[simp] theorem snd_pair : (pair a b).snd = b := rfl
+@[simp] theorem toPair_nil : nil.toPair = pair nil nil := rfl
+@[simp] theorem toPair_pair : (pair a b).toPair = pair a b := rfl
+@[simp] theorem ite_nil : ite nil a b = b := rfl
+@[simp] theorem ite_pair : ite (pair a b) c d = c := rfl
+@[simp] theorem ite_toPair : ite a.toPair b c = b := rfl
+@[simp] theorem not_isNil_T : ¬T.isNil := by simp [T]
+@[simp] theorem isNil_F : F.isNil := trivial
+@[simp] theorem isPair_T : T := trivial
+@[simp] theorem not_F : ¬F := by simp [F]
+@[simp] theorem not_nil_and : ¬nil.and a := by simp [and]
+@[simp] theorem isPair_toPair : a.toPair := trivial
+@[simp] theorem toProp_nil : nil.toProp = F := rfl
+@[simp] theorem toProp_pair : (pair a b).toProp = T := rfl
+@[simp] theorem isPair_toProp : a.toProp ↔ a := by cases a <;> simp
+@[simp] theorem and_iff : a.and b ↔ a ∧ b := by cases a <;> simp [and]
+
+theorem cases {p : Expr → Expr → Expr} {f : Expr → Expr}
+(h : ∀ x, (p x nil).and # p x (f x).toPair) : ∀ x, p x (f x) := by
+  intro x; simp at h; choose h₁ h₂ using h x; cases h : f x <;> simp_all
+
+theorem ind {p : Expr → Expr} (h : ∀ (x : Expr), (p nil).and # p x.toPair) : ∀ x, p x := by
+  intro x; simp at h; choose h₁ h₂ using h x; cases x <;> simp_all
+
+@[simp]
+theorem eq_iff : a.eq b ↔ a = b := by
+  simp [eq]; split_ifs <;> simp_all
+
+theorem le_def : a ≤ b ↔ a.sle b := by rfl
+theorem lt_def : a < b ↔ a.slt b := by rfl
+
+@[simp]
+theorem le_refl : a ≤ a := by
+  rw [le_def]; unfold sle; simp
+
+@[simp]
+theorem not_lt_nil : ¬a < nil := by
+  simp [lt_def, slt]
+
+@[simp]
+theorem nil_le : nil ≤ a := by
+  simp [le_def, sle]
+
+@[simp]
+theorem or_iff : a.or b ↔ a ∨ b := by
+  cases a <;> simp [or]
+
+@[simp]
+theorem nil_lt_iff : nil < a ↔ a := by
+  rw [lt_def]; unfold slt; split <;> simp [←le_def]
+
+@[simp]
+theorem pair_ne_fst : pair a b ≠ a := by
+  apply ne_of_congr sizeOf; simp; omega
+
+@[simp]
+theorem pair_ne_snd : pair a b ≠ b := by
+  apply ne_of_congr sizeOf; simp
+
+@[simp]
+theorem fst_ne_pair : a ≠ pair a b := by
+  simp [ne_symm']
+
+@[simp]
+theorem snd_ne_pair : b ≠ pair a b := by
+  simp [ne_symm']
+
+@[simp] theorem depth'_nil : nil.depth' = 0 := rfl
+@[simp] theorem depth'_pair : (pair a b).depth' = 1 + max a.depth' b.depth' := rfl
+
+@[simp]
+theorem depth'_eq_zero_iff : a.depth' = 0 ↔ a = nil := by
+  cases a <;> simp
+
+theorem depth'_le_of_le (h : a ≤ b) : a.depth' ≤ b.depth' := by
+  induction b
+  · simp
+    rw [le_def] at h; unfold sle at h
+    split_ifs at h <;> simp_all
+  nm x y ih₁ ih₂
+  simp
+  rw [le_def] at h; unfold sle at h
+  split_ifs at h with h₁
+  · simp [h₁]
+  split at h
+  · simp
+  · simp at h
+  nm q w e r z h₂ h₃
+  simp at h₃
+  obtain ⟨rfl, rfl⟩ := h₃
+  simp at h
+  grind [le_def]
+
+@[simp]
+theorem not_pair_le_fst : ¬pair a b ≤ a := by
+  intro h; replace h := depth'_le_of_le h; simp at h; omega
+
+@[simp]
+theorem not_pair_le_snd : ¬pair a b ≤ b := by
+  intro h; replace h := depth'_le_of_le h; simp at h; omega
+
+@[simp]
+theorem lt_irrefl : ¬a < a := by
+  rw [lt_def]; unfold slt; split <;> simp [←le_def]
+
+theorem not_pair_le_nil : ¬pair a b ≤ nil := by
+  simp [le_def, sle]
+
+@[simp]
+theorem le_nil_iff : a ≤ nil ↔ a = nil := by
+  cases a <;> simp [not_pair_le_nil]
+
+theorem le_iff_eq_or_lt : a ≤ b ↔ a = b ∨ a < b := by
+  simp [lt_def, slt]; cases b <;> simp; nm x y
+  conv => left; rw [le_def]; unfold sle
+  split_ifs <;> simp_all; split <;> simp_all [←le_def]
+
+theorem lt_iff_le_and_ne : a < b ↔ a ≤ b ∧ ¬a.eq b := by
+  simp [le_iff_eq_or_lt]
+  symm; use by grind
+  intro h; by_cases h₁ : a = b
+  on_goal 2 => grind
+  subst h₁; simp at h
+
+theorem le_of_lt (h : a < b) : a ≤ b := by
+  rw [le_iff_eq_or_lt]; tauto
+
+@[simp]
+theorem lt_pair_iff : a < pair b c ↔ a ≤ b ∨ a ≤ c := by
+  rw [lt_def, slt]; simp [←le_def]
+
+theorem depth'_lt_of_lt (h : a < b) : a.depth' < b.depth' := by
+  simp [lt_iff_le_and_ne] at h
+  choose h₁ h₂ using h
+  induction b
+  · simp [h₂] at h₁
+  nm x y ih₁ ih₂
+  simp
+  simp [le_iff_eq_or_lt, h₂] at h₁
+  simp [←le_iff_eq_or_lt] at h₁
+  grind
+
+theorem depth'_le_of_lt (h : a < b) : a.depth' ≤ b.depth' :=
+  Nat.le_of_lt # depth'_lt_of_lt h
+
+@[simp]
+theorem not_pair_lt_fst : ¬pair a b < a := by
+  intro h; replace h := depth'_lt_of_lt h; simp at h; omega
+
+@[simp]
+theorem not_pair_lt_snd : ¬pair a b < b := by
+  intro h; replace h := depth'_lt_of_lt h; simp at h; omega
+
+-----
+
+-- instance : WellFoundedRelation Expr where
+--   rel a b := a < b
+--   wf := by sorry
+
+-- def fn (fs : List (Expr → Expr)) (f : (Expr → Expr) → (x : Expr) → Expr) (x : Expr) : Expr :=
+--   let xs : List Expr := fs.map (· x)
+--   f (x := x) λ y =>
+--     let ys := fs.map (· y)
+--     if h : ys < xs then fn fs f y else nil
+-- termination_by fs.map (· x)
+-- decreasing_by
+
+-- def f (n m : ℕ) : ℕ :=
+--   match n, m with
+--   | 0, 0 => 0
+--   | 0, m + 1 => f 0 m
+--   | n + 1, 0 => f n (n ^ 2)
+--   | n + 1, m + 1 => f (n + 1) m
+-- termination_by ![n, m]
+-- decreasing_by
+
+-----
+
+-- def isTree (e : Expr) : Expr
