Projects/Expr/Defs.lean
@@ -1,0 +1,86 @@
+import Projects.Util
+
+inductive Expr where
+| nil : Expr
+| pair : Expr → Expr → Expr
+deriving Inhabited, DecidableEq
+
+namespace Expr
+
+variable {a b c : Expr}
+
+def isNil (a : Expr) : Prop :=
+  match a with | .nil => True | _ => False
+
+def isPair (a : Expr) : Prop :=
+  match a with | .nil => False | _ => True
+
+instance : Decidable (isNil a) :=
+  match a with
+  | .nil => .isTrue # by simp [isNil]
+  | pair _ _ => .isFalse # by simp [isNil]
+
+instance : Decidable (isPair a) :=
+  match a with
+  | .nil => .isFalse # by simp [isPair]
+  | pair _ _ => .isTrue # by simp [isPair]
+
+instance : CoeSort Expr Prop := ⟨isPair⟩
+
+def fst (a : Expr) : Expr :=
+  match a with | .nil => .nil | .pair a _ => a
+
+def snd (a : Expr) : Expr :=
+  match a with | .nil => .nil | .pair _ b => b
+
+def toPair (a : Expr) : Expr :=
+  .pair a.fst a.snd
+
+def ite (a b c : Expr) : Expr :=
+  if a.isPair then b else c
+
+def T : Expr := pair nil nil
+def F : Expr := nil
+
+def toProp (a : Expr) : Expr :=
+  ite a T F
+
+def not (a : Expr) : Expr :=
+  ite a F T
+
+def imp (a b : Expr) : Expr :=
+  ite a (toProp b) T
+
+def or (a b : Expr) : Expr :=
+  ite a T (toProp b)
+
+def and (a b : Expr) : Expr :=
+  ite a (toProp b) F
+
+def iff (a b : Expr) : Expr :=
+  ite a (toProp b) (not b)
+
+def eq (a b : Expr) : Expr :=
+  if a = b then T else F
+
+def sle (a b : Expr) : Expr :=
+  if a = b then T else match a, b with
+  | nil, _ => T
+  | _, nil => F
+  | _, pair x y => a.sle x |>.or # a.sle y
+  
+def slt (a b : Expr) : Expr :=
+  match b with
+  | nil => F
+  | pair c d => (sle a c).or (sle a d)
+
+def depth' (a : Expr) : ℕ :=
+  match a with
+  | nil => 0
+  | pair x y => 1 + max x.depth' y.depth'
+
+instance : LE Expr := ⟨λ a b => a.sle b⟩
+instance : LT Expr := ⟨λ a b => a.slt b⟩
+
+instance : DecidableLE Expr := λ a b => inferInstanceAs(Decidable # a.sle b)
+instance : DecidableLT Expr := λ a b => inferInstanceAs(Decidable # a.slt b)
